Fully monadic interpreter that extracts.

theories/safety.v
@@ -10,33 +10,46 @@ Unset Printing Implicit Defensive.
 
 Require Import operations typing type_checker opsem.
 
-Lemma progress :
-  forall i s vs es ts,
+
+Section Host.
+
+Variable host_function : eqType.
+Variable host_instance : host host_function.
+
+Let host_state := host_state host_instance.
+Let store_record := store_record host_function.
+Let administrative_instruction := administrative_instruction host_function.
+Let reduce := @reduce _ host_instance.
+
+Lemma progress : forall i s vs es ts hs,
   config_typing i s vs es ts ->
   const_list es \/
   es = [::Trap] \/
-  (exists s' vs' es', reduce s vs es i s' vs' es').
+  (exists s' vs' es' hs', reduce hs s vs es i hs' s' vs' es').
 Admitted. (* TODO *)
 
-Lemma preservation :
-  forall i s vs es ts s' vs' es',
+Lemma preservation : forall i s vs es ts s' vs' es' hs hs',
   config_typing i s vs es ts ->
-  reduce s vs es i s' vs' es' ->
+  reduce hs s vs es i hs' s' vs' es' ->
   config_typing i s' vs' es' ts.
 Admitted. (* TODO *)
 
-Inductive reduce_star : store_record -> list value -> list administrative_instruction -> instance -> store_record -> list value -> list administrative_instruction -> Prop :=
-| reduce_refl : forall s vs es i, reduce_star s vs es i s vs es
-| reduce_step : forall s vs es i s' vs' es' s'' vs'' es'',
-    reduce s vs es i s' vs' es' ->
-    reduce_star s' vs' es' i s'' vs'' es'' ->
-    reduce_star s vs es i s'' vs'' es''.
+Inductive reduce_star : host_state -> store_record -> list value -> list administrative_instruction -> instance ->
+                        host_state -> store_record -> list value -> list administrative_instruction -> Prop :=
+  | reduce_refl : forall hs s vs es i, reduce_star hs s vs es i hs s vs es
+  | reduce_step : forall hs s vs es i hs' s' vs' es' hs'' s'' vs'' es'',
+    reduce hs s vs es i hs' s' vs' es' ->
+    reduce_star hs' s' vs' es' i hs'' s'' vs'' es'' ->
+    reduce_star hs s vs es i hs'' s'' vs'' es''
+  .
 
-Lemma safety :
-  forall i s vs es ts,
+Lemma safety : forall hs i s vs es ts,
     config_typing i s vs es ts ->
-    (exists s' vs' es', (const_list es' \/ es' = [::Trap]) /\ reduce_star s vs es i s' vs' es') \/
-    (exists sn vsn esn, sn 0 = s /\ vsn 0 = vs /\ esn 0 = es /\
-                        forall n, reduce (sn n) (vsn n) (esn n) i (sn n.+1) (vsn n.+1) (esn n.+1)).
+    (exists s' vs' es' hs',
+      (const_list es' \/ es' = [::Trap]) /\ reduce_star hs s vs es i hs' s' vs' es') \/
+    (exists hsn sn vsn esn, hsn 0 = hs /\ sn 0 = s /\ vsn 0 = vs /\ esn 0 = es /\
+      forall n, reduce (hsn n) (sn n) (vsn n) (esn n) i (hsn n.+1) (sn n.+1) (vsn n.+1) (esn n.+1)).
 Admitted. (* TODO *)
+
+End Host.
 
