theories/interpreter.v
@@ -21,8 +21,13 @@ Let monadic_host := monadic_host host_function.
 
 Variable host_instance : monadic_host.
 
-Let host_return := host_return host_instance.
-Let host_apply := host_apply host_instance.
+Let host_monad := host_monad host_instance.
+Let host_return : forall A, A -> host_monad A :=
+  host_return host_instance.
+Let host_bind : forall A B, host_monad A -> (A -> host_monad B) -> host_monad B :=
+  host_bind host_instance.
+Let host_apply : store_record -> host_function -> seq value -> host_monad (option (store_record * result)) :=
+  host_apply host_instance.
 
 
 (** * Types used by the interpreter **)
@@ -78,16 +83,16 @@ Definition depth := nat.
   but relying on fuel. **)
 Definition fuel := nat.
 
-Definition config_tuple := ((store_record * seq value * seq administrative_instruction)%type).
+Definition config_tuple : Type := store_record * seq value * seq administrative_instruction.
 
-Definition config_one_tuple_without_e := (store_record * seq value * seq value)%type.
+Definition config_one_tuple_without_e : Type := store_record * seq value * seq value.
 
-Definition res_tuple := (store_record * seq value * res_step)%type.
+Definition res_tuple : Type := store_record * seq value * res_step.
 
 
 (** * The interpreter itself. **)
 
-Fixpoint split_vals (es : seq basic_instruction) : (seq value * seq basic_instruction)%type :=
+Fixpoint split_vals (es : seq basic_instruction) : seq value * seq basic_instruction :=
   match es with
   | (EConst v) :: es' =>
     let: (vs', es'') := split_vals es' in
@@ -99,7 +104,7 @@ Fixpoint split_vals (es : seq basic_instruction) : (seq value * seq basic_instru
     are all of the form [Basic (EConst v)];
     returns a pair of lists [(ves, es')] where [ves] are those [v]'s in that initial
     segment and [es] is the remainder of the original [es]. **)
-Fixpoint split_vals_e (es : seq administrative_instruction) : ((seq value) * (seq administrative_instruction))%type :=
+Fixpoint split_vals_e (es : seq administrative_instruction) : seq value * seq administrative_instruction :=
   match es with
   | (Basic (EConst v)) :: es' =>
     let: (vs', es'') := split_vals_e es' in
@@ -107,7 +112,7 @@ Fixpoint split_vals_e (es : seq administrative_instruction) : ((seq value) * (se
   | _ => ([::], es)
   end.
 
-Fixpoint split_n (es : seq value) (n : nat) : (seq value * seq value)%type :=
+Fixpoint split_n (es : seq value) (n : nat) : seq value * seq value :=
   match (es, n) with
   | ([::], _) => ([::], [::])
   | (_, 0) => ([::], es)
@@ -152,218 +157,227 @@ Proof.
   - move=> >. by apply: ReflectF.
 Qed.
 
-Fixpoint run_step_with_fuel (fuel : fuel) (d : depth) (i : instance) (tt : config_tuple) : res_tuple :=
+Fixpoint run_step_with_fuel (fuel : fuel) (d : depth) (i : instance) (tt : config_tuple)
+    : host_monad res_tuple :=
   let: (s, vs, es) := tt in
   match fuel with
-  | 0 => (s, vs, RS_crash C_exhaustion)
+  | 0 => host_return (s, vs, RS_crash C_exhaustion)
   | fuel.+1 =>
     let: (ves, es') := split_vals_e es in (** Framing out constants. **)
     match es' with
-    | [::] => (s, vs, crash_error)
+    | [::] => host_return (s, vs, crash_error)
     | e :: es'' =>
       if e_is_trap e
       then
         if (es'' != [::]) || (ves != [::])
-        then (s, vs, RS_normal [::Trap])
-        else (s, vs, crash_error)
+        then host_return (s, vs, RS_normal [::Trap])
+        else host_return (s, vs, crash_error)
       else
-        let: (s', vs', r) := run_one_step fuel d i (s, vs, (rev ves)) e in
-        if r is RS_normal res
-        then (s', vs', RS_normal (res ++ es''))
-        else (s', vs', r)
+        host_bind (run_one_step fuel d i (s, vs, (rev ves)) e) (fun rosf =>
+          let: (s', vs', r) := rosf in
+          if r is RS_normal res
+          then host_return (s', vs', RS_normal (res ++ es''))
+          else host_return (s', vs', r))
     end
   end
 
-with run_one_step (fuel : fuel) (d : depth) (i : instance) (tt : config_one_tuple_without_e) (e : administrative_instruction) : res_tuple :=
+with run_one_step (fuel : fuel) (d : depth) (i : instance) (tt : config_one_tuple_without_e) (e : administrative_instruction)
+    : host_monad res_tuple :=
   let: (s, vs, ves) := tt in
   match fuel with
-  | 0 => (s, vs, RS_crash C_exhaustion)
+  | 0 => host_return (s, vs, RS_crash C_exhaustion)
   | fuel.+1 =>
     match e with
-    (* unop *)
+
+    (** unop **)
     | Basic (Unop_i T_i32 iop) =>
       if ves is ConstInt32 c :: ves' then
-        (s, vs, RS_normal (vs_to_es ((ConstInt32 (@app_unop_i i32t iop c)) :: ves')))
-      else (s, vs, crash_error)
+        host_return (s, vs, RS_normal (vs_to_es ((ConstInt32 (@app_unop_i i32t iop c)) :: ves')))
+      else host_return (s, vs, crash_error)
     | Basic (Unop_i T_i64 iop) =>
       if ves is (ConstInt64 c) :: ves' then
-        (s, vs, RS_normal (vs_to_es ((ConstInt64 (@app_unop_i i64t iop c)) :: ves')))
-      else (s, vs, crash_error)
-    | Basic (Unop_i _ _) => (s, vs, crash_error)
+        host_return (s, vs, RS_normal (vs_to_es ((ConstInt64 (@app_unop_i i64t iop c)) :: ves')))
+      else host_return (s, vs, crash_error)
+    | Basic (Unop_i _ _) => host_return (s, vs, crash_error)
     | Basic (Unop_f T_f32 iop) =>
       if ves is (ConstFloat32 c) :: ves' then
-        (s, vs, RS_normal (vs_to_es ((ConstFloat32 (@app_unop_f f32t iop c)) :: ves')))
-      else (s, vs, crash_error)
+        host_return (s, vs, RS_normal (vs_to_es ((ConstFloat32 (@app_unop_f f32t iop c)) :: ves')))
+      else host_return (s, vs, crash_error)
     | Basic (Unop_f T_f64 iop) =>
       if ves is (ConstFloat64 c) :: ves' then
-        (s, vs, RS_normal (vs_to_es ((ConstFloat64 (@app_unop_f f64t iop c)) :: ves')))
-      else (s, vs, crash_error)
-    | Basic (Unop_f _ _) => (s, vs, crash_error)
-    (* binop *)
+        host_return (s, vs, RS_normal (vs_to_es ((ConstFloat64 (@app_unop_f f64t iop c)) :: ves')))
+      else host_return (s, vs, crash_error)
+    | Basic (Unop_f _ _) => host_return (s, vs, crash_error)
+
+    (** binop **)
     | Basic (Binop_i T_i32 iop) =>
       if ves is (ConstInt32 c2) :: (ConstInt32 c1) :: ves' then
         expect (@app_binop_i i32t iop c1 c2) (fun c =>
-            (s, vs, RS_normal (vs_to_es ((ConstInt32 c) :: ves'))))
-          (s, vs, RS_normal ((vs_to_es ves') ++ [::Trap]))
-      else (s, vs, crash_error)
+            host_return (s, vs, RS_normal (vs_to_es ((ConstInt32 c) :: ves'))))
+          (host_return (s, vs, RS_normal ((vs_to_es ves') ++ [::Trap])))
+      else host_return (s, vs, crash_error)
     | Basic (Binop_i T_i64 iop) =>
       if ves is (ConstInt64 c2) :: (ConstInt64 c1) :: ves' then
         expect (@app_binop_i i64t iop c1 c2) (fun c =>
-            (s, vs, RS_normal (vs_to_es ((ConstInt64 c) :: ves'))))
-          (s, vs, RS_normal ((vs_to_es ves') ++ [::Trap]))
-      else (s, vs, crash_error)
-    | Basic (Binop_i _ _) => (s, vs, crash_error)
+            host_return (s, vs, RS_normal (vs_to_es ((ConstInt64 c) :: ves'))))
+          (host_return (s, vs, RS_normal ((vs_to_es ves') ++ [::Trap])))
+      else host_return (s, vs, crash_error)
+    | Basic (Binop_i _ _) => host_return (s, vs, crash_error)
     | Basic (Binop_f T_f32 fop) =>
       if ves is (ConstFloat32 c2) :: (ConstFloat32 c1) :: ves' then
         expect (@app_binop_f f32t fop c1 c2) (fun c =>
-            (s, vs, RS_normal (vs_to_es ((ConstFloat32 c) :: ves'))))
-          (s, vs, RS_normal ((vs_to_es ves') ++ [::Trap]))
-      else (s, vs, crash_error)
+            host_return (s, vs, RS_normal (vs_to_es ((ConstFloat32 c) :: ves'))))
+          (host_return (s, vs, RS_normal ((vs_to_es ves') ++ [::Trap])))
+      else host_return (s, vs, crash_error)
     | Basic (Binop_f T_f64 fop) =>
       if ves is (ConstFloat64 c2) :: (ConstFloat64 c1) :: ves' then
         expect (@app_binop_f f64t fop c1 c2) (fun c =>
-             (s, vs, RS_normal (vs_to_es ((ConstFloat64 c) :: ves'))))
-          (s, vs, RS_normal ((vs_to_es ves') ++ [::Trap]))
-      else (s, vs, crash_error)
-    | Basic (Binop_f _ _) => (s, vs, crash_error)
-    (* testops *)
+             host_return (s, vs, RS_normal (vs_to_es ((ConstFloat64 c) :: ves'))))
+          (host_return (s, vs, RS_normal ((vs_to_es ves') ++ [::Trap])))
+      else host_return (s, vs, crash_error)
+    | Basic (Binop_f _ _) => host_return (s, vs, crash_error)
+
+    (** testops **)
     | Basic (Testop T_i32 testop) =>
       if ves is (ConstInt32 c) :: ves' then
-        (s, vs, RS_normal (vs_to_es ((ConstInt32 (wasm_bool (@app_testop_i i32t testop c))) :: ves')))
-      else (s, vs, crash_error)
+        host_return (s, vs, RS_normal (vs_to_es ((ConstInt32 (wasm_bool (@app_testop_i i32t testop c))) :: ves')))
+      else host_return (s, vs, crash_error)
     | Basic (Testop T_i64 testop) =>
       if ves is (ConstInt64 c) :: ves' then
-        (s, vs, RS_normal (vs_to_es ((ConstInt32 (wasm_bool (@app_testop_i i64t testop c))) :: ves')))
-      else (s, vs, crash_error)
-    | Basic (Testop _ _) => (s, vs, crash_error)
-    (* relops *)
+        host_return (s, vs, RS_normal (vs_to_es ((ConstInt32 (wasm_bool (@app_testop_i i64t testop c))) :: ves')))
+      else host_return (s, vs, crash_error)
+    | Basic (Testop _ _) => host_return (s, vs, crash_error)
+
+    (** relops **)
     | Basic (Relop_i T_i32 iop) =>
       if ves is (ConstInt32 c2) :: (ConstInt32 c1) :: ves' then
-        (s, vs, RS_normal (vs_to_es (ConstInt32 (wasm_bool (@app_relop_i i32t iop c1 c2)) :: ves')))
-      else (s, vs, crash_error)
+        host_return (s, vs, RS_normal (vs_to_es (ConstInt32 (wasm_bool (@app_relop_i i32t iop c1 c2)) :: ves')))
+      else host_return (s, vs, crash_error)
     | Basic (Relop_i T_i64 iop) =>
       if ves is (ConstInt64 c2) :: (ConstInt64 c1) :: ves' then
-        (s, vs, RS_normal (vs_to_es (ConstInt32 (wasm_bool (@app_relop_i i64t iop c1 c2)) :: ves')))
-      else (s, vs, crash_error)
-    | Basic (Relop_i _ _) => (s, vs, crash_error)
+        host_return (s, vs, RS_normal (vs_to_es (ConstInt32 (wasm_bool (@app_relop_i i64t iop c1 c2)) :: ves')))
+      else host_return (s, vs, crash_error)
+    | Basic (Relop_i _ _) => host_return (s, vs, crash_error)
     | Basic (Relop_f T_f32 iop) =>
       if ves is (ConstFloat32 c2) :: (ConstFloat32 c1) :: ves' then
-        (s, vs, RS_normal (vs_to_es (ConstInt32 (wasm_bool (@app_relop_f f32t iop c1 c2)) :: ves')))
-      else (s, vs, crash_error)
+        host_return (s, vs, RS_normal (vs_to_es (ConstInt32 (wasm_bool (@app_relop_f f32t iop c1 c2)) :: ves')))
+      else host_return (s, vs, crash_error)
     | Basic (Relop_f T_f64 iop) =>
       if ves is (ConstFloat64 c2) :: (ConstFloat64 c1) :: ves' then
-        (s, vs, RS_normal (vs_to_es (ConstInt32 (wasm_bool (@app_relop_f f64t iop c1 c2)) :: ves')))
-      else (s, vs, crash_error)
-    | Basic (Relop_f _ _) => (s, vs, crash_error)
-    (* convert & reinterpret *)
+        host_return (s, vs, RS_normal (vs_to_es (ConstInt32 (wasm_bool (@app_relop_f f64t iop c1 c2)) :: ves')))
+      else host_return (s, vs, crash_error)
+    | Basic (Relop_f _ _) => host_return (s, vs, crash_error)
+
+    (** convert and reinterpret **)
     | Basic (Cvtop t2 Convert t1 sx) =>
       if ves is v :: ves' then
         if types_agree t1 v
         then
           expect (cvt t2 sx v) (fun v' =>
-               (s, vs, RS_normal (vs_to_es (v' :: ves'))))
-            (s, vs, RS_normal ((vs_to_es ves') ++ [::Trap]))
-        else (s, vs, crash_error)
-      else (s, vs, crash_error)
+               host_return (s, vs, RS_normal (vs_to_es (v' :: ves'))))
+            (host_return (s, vs, RS_normal ((vs_to_es ves') ++ [::Trap])))
+        else host_return (s, vs, crash_error)
+      else host_return (s, vs, crash_error)
     | Basic (Cvtop t2 Reinterpret t1 sx) =>
       if ves is v :: ves' then
         if types_agree t1 v && (sx == None)
-        then (s, vs, RS_normal (vs_to_es (wasm_deserialise (bits v) t2 :: ves')))
-        else (s, vs, crash_error)
-      else (s, vs, crash_error)
-    (**)
-    | Basic Unreachable => (s, vs, RS_normal ((vs_to_es ves) ++ [::Trap]))
-    | Basic Nop => (s, vs, RS_normal (vs_to_es ves))
+        then host_return (s, vs, RS_normal (vs_to_es (wasm_deserialise (bits v) t2 :: ves')))
+        else host_return (s, vs, crash_error)
+      else host_return (s, vs, crash_error)
+
+    (** control-flow instructions **)
+    | Basic Unreachable => host_return (s, vs, RS_normal ((vs_to_es ves) ++ [::Trap]))
+    | Basic Nop => host_return (s, vs, RS_normal (vs_to_es ves))
     | Basic Drop =>
       if ves is v :: ves' then
-        (s, vs, RS_normal (vs_to_es ves'))
-      else (s, vs, crash_error)
+        host_return (s, vs, RS_normal (vs_to_es ves'))
+      else host_return (s, vs, crash_error)
     | Basic Select =>
       if ves is (ConstInt32 c) :: v2 :: v1 :: ves' then
         if c == Wasm_int.int_zero i32m
-        then (s, vs, RS_normal (vs_to_es (v2 :: ves')))
-        else (s, vs, RS_normal (vs_to_es (v1 :: ves')))
-      else (s, vs, crash_error)
+        then host_return (s, vs, RS_normal (vs_to_es (v2 :: ves')))
+        else host_return (s, vs, RS_normal (vs_to_es (v1 :: ves')))
+      else host_return (s, vs, crash_error)
     | Basic (Block (Tf t1s t2s) es) =>
       if length ves >= length t1s
       then
         let: (ves', ves'')  := split_n ves (length t1s) in
-        (s, vs, RS_normal (vs_to_es ves''
-                ++ [::Label (length t2s) [::] (vs_to_es ves' ++ to_e_list es)]))
-      else (s, vs, crash_error)
+        host_return (s, vs, RS_normal (vs_to_es ves''
+                              ++ [::Label (length t2s) [::] (vs_to_es ves' ++ to_e_list es)]))
+      else host_return (s, vs, crash_error)
     | Basic (Loop (Tf t1s t2s) es) =>
       if length ves >= length t1s
       then
         let: (ves', ves'') := split_n ves (length t1s) in
-        (s, vs, RS_normal (vs_to_es ves''
-                ++ [::Label (length t1s) [::Basic (Loop (Tf t1s t2s) es)]
-                        (vs_to_es ves' ++ to_e_list es)]))
-      else (s, vs, crash_error)
+        host_return (s, vs, RS_normal (vs_to_es ves''
+                              ++ [::Label (length t1s) [::Basic (Loop (Tf t1s t2s) es)]
+                                      (vs_to_es ves' ++ to_e_list es)]))
+      else host_return (s, vs, crash_error)
     | Basic (If tf es1 es2) =>
       if ves is ConstInt32 c :: ves' then
         if c == Wasm_int.int_zero i32m
-        then (s, vs, RS_normal (vs_to_es ves' ++ [::Basic (Block tf es2)]))
-        else (s, vs, RS_normal (vs_to_es ves' ++ [::Basic (Block tf es1)]))
-      else (s, vs, crash_error)
-    | Basic (Br j) => (s, vs, RS_break j ves)
+        then host_return (s, vs, RS_normal (vs_to_es ves' ++ [::Basic (Block tf es2)]))
+        else host_return (s, vs, RS_normal (vs_to_es ves' ++ [::Basic (Block tf es1)]))
+      else host_return (s, vs, crash_error)
+    | Basic (Br j) => host_return (s, vs, RS_break j ves)
     | Basic (Br_if j) =>
       if ves is ConstInt32 c :: ves' then
         if c == Wasm_int.int_zero i32m
-        then (s, vs, RS_normal (vs_to_es ves'))
-        else (s, vs, RS_normal (vs_to_es ves' ++ [::Basic (Br j)]))
-      else (s, vs, crash_error)
+        then host_return (s, vs, RS_normal (vs_to_es ves'))
+        else host_return (s, vs, RS_normal (vs_to_es ves' ++ [::Basic (Br j)]))
+      else host_return (s, vs, crash_error)
     | Basic (Br_table js j) =>
       if ves is ConstInt32 c :: ves' then
         let: k := Wasm_int.nat_of_uint i32m c in
         if k < length js
         then
-          expect (List.nth_error js k) (fun js_at_k =>
+          host_return (expect (List.nth_error js k) (fun js_at_k =>
               (s, vs, RS_normal (vs_to_es ves' ++ [::Basic (Br js_at_k)])))
-            (s, vs, crash_error)
-        else (s, vs, RS_normal (vs_to_es ves' ++ [::Basic (Br j)]))
-      else (s, vs, crash_error)
+            (s, vs, crash_error))
+        else host_return (s, vs, RS_normal (vs_to_es ves' ++ [::Basic (Br j)]))
+      else host_return (s, vs, crash_error)
     | Basic (Call j) =>
       if sfunc s i j is Some sfunc_i_j then
-        (s, vs, RS_normal (vs_to_es ves ++ [::Callcl sfunc_i_j]))
-      else (s, vs, crash_error)
+        host_return (s, vs, RS_normal (vs_to_es ves ++ [::Callcl sfunc_i_j]))
+      else host_return (s, vs, crash_error)
     | Basic (Call_indirect j) =>
       if ves is ConstInt32 c :: ves' then
         match stab s i (Wasm_int.nat_of_uint i32m c) with
         | Some cl =>
           if stypes s i j == Some (cl_type cl)
-          then (s, vs, RS_normal (vs_to_es ves' ++ [::Callcl cl]))
-          else (s, vs, RS_normal (vs_to_es ves' ++ [::Trap]))
-        | None => (s, vs, RS_normal (vs_to_es ves' ++ [::Trap]))
+          then host_return (s, vs, RS_normal (vs_to_es ves' ++ [::Callcl cl]))
+          else host_return (s, vs, RS_normal (vs_to_es ves' ++ [::Trap]))
+        | None => host_return (s, vs, RS_normal (vs_to_es ves' ++ [::Trap]))
         end
-      else (s, vs, crash_error)
-    | Basic Return => (s, vs, RS_return ves)
+      else host_return (s, vs, crash_error)
+    | Basic Return => host_return (s, vs, RS_return ves)
     | Basic (Get_local j) =>
       if j < length vs
       then
-        expect (List.nth_error vs j) (fun vs_at_j =>
+        host_return (expect (List.nth_error vs j) (fun vs_at_j =>
             (s, vs, RS_normal (vs_to_es (vs_at_j :: ves))))
-          (s, vs, crash_error)
-      else (s, vs, crash_error)
+          (s, vs, crash_error))
+      else host_return (s, vs, crash_error)
     | Basic (Set_local j) =>
       if ves is v :: ves' then
         if j < length vs
-        then (s, update_list_at vs j v, RS_normal (vs_to_es ves'))
-        else (s, vs, crash_error)
-      else (s, vs, crash_error)
+        then host_return (s, update_list_at vs j v, RS_normal (vs_to_es ves'))
+        else host_return (s, vs, crash_error)
+      else host_return (s, vs, crash_error)
     | Basic (Tee_local j) =>
       if ves is v :: ves' then
-        (s, vs, RS_normal (vs_to_es (v :: ves) ++ [::Basic (Set_local j)]))
-      else (s, vs, crash_error)
+        host_return (s, vs, RS_normal (vs_to_es (v :: ves) ++ [::Basic (Set_local j)]))
+      else host_return (s, vs, crash_error)
     | Basic (Get_global j) =>
       if sglob_val s i j is Some xx
-      then (s, vs, RS_normal (vs_to_es (xx :: ves)))
-      else (s, vs, crash_error)
+      then host_return (s, vs, RS_normal (vs_to_es (xx :: ves)))
+      else host_return (s, vs, crash_error)
     | Basic (Set_global j) =>
       if ves is v :: ves' then
         if supdate_glob s i j v is Some xx
-        then (xx, vs, RS_normal (vs_to_es ves'))
-        else (s, vs, crash_error)
-      else (s, vs, crash_error)
+        then host_return (xx, vs, RS_normal (vs_to_es ves'))
+        else host_return (s, vs, crash_error)
+      else host_return (s, vs, crash_error)
     | Basic (Load t None a off) =>
       if ves is ConstInt32 k :: ves' then
         expect
@@ -372,11 +386,12 @@ with run_one_step (fuel : fuel) (d : depth) (i : instance) (tt : config_one_tupl
              if List.nth_error (s_memory s) j is Some mem_s_j then
                expect
                  (load (mem_s_j) (Wasm_int.nat_of_uint i32m k) off (t_length t))
-                 (fun bs => (s, vs, RS_normal (vs_to_es (wasm_deserialise bs t :: ves'))))
-                 (s, vs, RS_normal (vs_to_es ves' ++ [::Trap]))
-             else (s, vs, crash_error))
-          (s, vs, crash_error)
-      else (s, vs, crash_error)
+                 (fun bs =>
+                    host_return (s, vs, RS_normal (vs_to_es (wasm_deserialise bs t :: ves'))))
+                 (host_return (s, vs, RS_normal (vs_to_es ves' ++ [::Trap])))
+             else host_return (s, vs, crash_error))
+          (host_return (s, vs, crash_error))
+      else host_return (s, vs, crash_error)
     | Basic (Load t (Some (tp, sx)) a off) =>
       if ves is ConstInt32 k :: ves' then
         expect
@@ -385,11 +400,12 @@ with run_one_step (fuel : fuel) (d : depth) (i : instance) (tt : config_one_tupl
              if List.nth_error (s_memory s) j is Some mem_s_j then
                expect
                  (load_packed sx (mem_s_j) (Wasm_int.nat_of_uint i32m k) off (tp_length tp) (t_length t))
-                 (fun bs => (s, vs, RS_normal (vs_to_es (wasm_deserialise bs t :: ves'))))
-                 (s, vs, RS_normal (vs_to_es ves' ++ [::Trap]))
-             else (s, vs, crash_error))
-          (s, vs, crash_error)
-      else (s, vs, crash_error)
+                 (fun bs =>
+                    host_return (s, vs, RS_normal (vs_to_es (wasm_deserialise bs t :: ves'))))
+                 (host_return (s, vs, RS_normal (vs_to_es ves' ++ [::Trap])))
+             else host_return (s, vs, crash_error))
+          (host_return (s, vs, crash_error))
+      else host_return (s, vs, crash_error)
     | Basic (Store t None a off) =>
       if ves is v :: ConstInt32 k :: ves' then
         if types_agree t v
@@ -401,12 +417,12 @@ with run_one_step (fuel : fuel) (d : depth) (i : instance) (tt : config_one_tupl
                  expect
                    (store mem_s_j (Wasm_int.nat_of_uint i32m k) off (bits v) (t_length t))
                    (fun mem' =>
-                      (upd_s_mem s (update_list_at (s_memory s) j mem'), vs, RS_normal (vs_to_es ves')))
-                   (s, vs, RS_normal (vs_to_es ves' ++ [::Trap]))
-               else (s, vs, crash_error))
-            (s, vs, crash_error)
-        else (s, vs, crash_error)
-      else (s, vs, crash_error)
+                      host_return (upd_s_mem s (update_list_at (s_memory s) j mem'), vs, RS_normal (vs_to_es ves')))
+                   (host_return (s, vs, RS_normal (vs_to_es ves' ++ [::Trap])))
+               else host_return (s, vs, crash_error))
+            (host_return (s, vs, crash_error))
+        else host_return (s, vs, crash_error)
+      else host_return (s, vs, crash_error)
     | Basic (Store t (Some tp) a off) =>
       if ves is v :: ConstInt32 k :: ves' then
         if types_agree t v
@@ -418,20 +434,20 @@ with run_one_step (fuel : fuel) (d : depth) (i : instance) (tt : config_one_tupl
                  expect
                    (store_packed mem_s_j (Wasm_int.nat_of_uint i32m k) off (bits v) (tp_length tp))
                    (fun mem' =>
-                      (upd_s_mem s (update_list_at (s_memory s) j mem'), vs, RS_normal (vs_to_es ves')))
-                   (s, vs, RS_normal (vs_to_es ves' ++ [::Trap]))
-               else (s, vs, crash_error))
-            (s, vs, crash_error)
-        else (s, vs, crash_error)
-      else (s, vs, crash_error)
+                      host_return (upd_s_mem s (update_list_at (s_memory s) j mem'), vs, RS_normal (vs_to_es ves')))
+                   (host_return (s, vs, RS_normal (vs_to_es ves' ++ [::Trap])))
+               else host_return (s, vs, crash_error))
+            (host_return (s, vs, crash_error))
+        else host_return (s, vs, crash_error)
+      else host_return (s, vs, crash_error)
     | Basic Current_memory =>
       expect
         (smem_ind s i)
         (fun j =>
            if List.nth_error (s_memory s) j is Some s_mem_s_j then
-             (s, vs, RS_normal (vs_to_es (ConstInt32 (Wasm_int.int_of_Z i32m (Z.of_nat (mem_size s_mem_s_j))) :: ves)))
-           else (s, vs, crash_error))
-        (s, vs, crash_error)
+             host_return (s, vs, RS_normal (vs_to_es (ConstInt32 (Wasm_int.int_of_Z i32m (Z.of_nat (mem_size s_mem_s_j))) :: ves)))
+           else host_return (s, vs, crash_error))
+        (host_return (s, vs, crash_error))
     | Basic Grow_memory =>
       if ves is ConstInt32 c :: ves' then
         expect
@@ -440,12 +456,12 @@ with run_one_step (fuel : fuel) (d : depth) (i : instance) (tt : config_one_tupl
             if List.nth_error (s_memory s) j is Some s_mem_s_j then
               let: l := mem_size s_mem_s_j in
               let: mem' := mem_grow s_mem_s_j (Wasm_int.nat_of_uint i32m c) in
-              (upd_s_mem s (update_list_at (s_memory s) j mem'), vs,
-               RS_normal (vs_to_es (ConstInt32 (Wasm_int.int_of_Z i32m (Z.of_nat l)) :: ves')))
-            else (s, vs, crash_error))
-          (s, vs, crash_error)
-      else (s, vs, crash_error)
-    | Basic (EConst _) => (s, vs, crash_error)
+              let: s' := upd_s_mem s (update_list_at (s_memory s) j mem') in
+              host_return (s', vs, RS_normal (vs_to_es (ConstInt32 (Wasm_int.int_of_Z i32m (Z.of_nat l)) :: ves')))
+            else host_return (s, vs, crash_error))
+          (host_return (s, vs, crash_error))
+      else host_return (s, vs, crash_error)
+    | Basic (EConst _) => host_return (s, vs, crash_error)
     | Callcl cl =>
       match cl with
       | Func_native i' (Tf t1s t2s) ts es =>
@@ -455,71 +471,72 @@ with run_one_step (fuel : fuel) (d : depth) (i : instance) (tt : config_one_tupl
         then
           let: (ves', ves'') := split_n ves n in
           let: zs := n_zeros ts in
-          (s, vs, RS_normal (vs_to_es ves''
-                  ++ [::Local m i' (rev ves' ++ zs) [::Basic (Block (Tf [::] t2s) es)]]))
-        else (s, vs, crash_error)
+          host_return (s, vs, RS_normal (vs_to_es ves''
+                                ++ [::Local m i' (rev ves' ++ zs) [::Basic (Block (Tf [::] t2s) es)]]))
+        else host_return (s, vs, crash_error)
       | Func_host (Tf t1s t2s) f =>
         let: n := length t1s in
         let: m := length t2s in
         if length ves >= n
         then
           let: (ves', ves'') := split_n ves n in
-          host_apply s f (rev ves') (fun r =>
-            host_return
-              (match r with
-               | Some (s', r) =>
-                 (** We here double-check the types.
-                   Note that this is not a requirement of the Wasm specification. **)
-                 if result_types_agree t2s r
-                 then
-                   let: rves := result_to_stack r in
-                   (s', vs, RS_normal (vs_to_es ves'' ++ rves))
-                 else (s, vs, crash_error)
-               | None => (s, vs, crash_error) (* TODO *)
-               end))
-        else (s, vs, crash_error)
+          host_bind (host_apply s f (rev ves')) (fun r =>
+            match r with
+            | Some (s', r) =>
+              (** We here double-check the types.
+                Note that this is not a requirement of the Wasm specification. **)
+              if result_types_agree t2s r
+              then
+                let: rves := result_to_stack r in
+                host_return (s', vs, RS_normal (vs_to_es ves'' ++ rves))
+              else host_return (s, vs, crash_error)
+            | None => host_return (s, vs, crash_error) (* TODO *)
+            end)
+        else host_return (s, vs, crash_error)
       end
     | Label ln les es =>
       if es_is_trap es
-      then (s, vs, RS_normal (vs_to_es ves ++ [::Trap]))
+      then host_return (s, vs, RS_normal (vs_to_es ves ++ [::Trap]))
       else
         if const_list es
-        then (s, vs, RS_normal (vs_to_es ves ++ es))
+        then host_return (s, vs, RS_normal (vs_to_es ves ++ es))
         else
-          let: (s', vs', res) := run_step_with_fuel fuel d i (s, vs, es) in
-          match res with
-          | RS_break 0 bvs =>
-            if length bvs >= ln
-            then (s', vs', RS_normal ((vs_to_es ((take ln bvs) ++ ves)) ++ les))
-            else (s', vs', crash_error)
-          | RS_break (n.+1) bvs => (s', vs', RS_break n bvs)
-          | RS_return rvs => (s', vs', RS_return rvs)
-          | RS_normal es' =>
-            (s', vs', RS_normal (vs_to_es ves ++ [::Label ln les es']))
-          | RS_crash error => (s', vs', RS_crash error)
-          end
+          host_bind (run_step_with_fuel fuel d i (s, vs, es)) (fun rswf =>
+            let: (s', vs', res) := rswf in
+            match res with
+            | RS_break 0 bvs =>
+              if length bvs >= ln
+              then host_return (s', vs', RS_normal ((vs_to_es ((take ln bvs) ++ ves)) ++ les))
+              else host_return (s', vs', crash_error)
+            | RS_break (n.+1) bvs => host_return (s', vs', RS_break n bvs)
+            | RS_return rvs => host_return (s', vs', RS_return rvs)
+            | RS_normal es' =>
+              host_return (s', vs', RS_normal (vs_to_es ves ++ [::Label ln les es']))
+            | RS_crash error => host_return (s', vs', RS_crash error)
+            end)
     | Local ln j vls es =>
       if es_is_trap es
-      then (s, vs, RS_normal (vs_to_es ves ++ [::Trap]))
+      then host_return (s, vs, RS_normal (vs_to_es ves ++ [::Trap]))
       else
         if const_list es
         then
           if length es == ln
-          then (s, vs, RS_normal (vs_to_es ves ++ es))
-          else (s, vs, crash_error)
+          then host_return (s, vs, RS_normal (vs_to_es ves ++ es))
+          else host_return (s, vs, crash_error)
         else
-          let: (s', vls', res) := run_step_with_fuel fuel d j (s, vls, es) in
-          match res with
-          | RS_return rvs =>
-            if length rvs >= ln
-            then (s', vs, RS_normal (vs_to_es (take ln rvs ++ ves)))
-            else (s', vs, crash_error)
-          | RS_normal es' =>
-            (s', vs, RS_normal (vs_to_es ves ++ [::Local ln j vls' es']))
-          | RS_crash error => (s', vs, RS_crash error)
-          | RS_break _ _ => (s', vs, crash_error)
-          end
-    | Trap => (s, vs, crash_error)
+          host_bind (run_step_with_fuel fuel d j (s, vls, es)) (fun rswf =>
+            let: (s', vls', res) := rswf in
+            match res with
+            | RS_return rvs =>
+              if length rvs >= ln
+              then host_return (s', vs, RS_normal (vs_to_es (take ln rvs ++ ves)))
+              else host_return (s', vs, crash_error)
+            | RS_normal es' =>
+              host_return (s', vs, RS_normal (vs_to_es ves ++ [::Local ln j vls' es']))
+            | RS_crash error => host_return (s', vs, RS_crash error)
+            | RS_break _ _ => host_return (s', vs, crash_error)
+            end)
+    | Trap => host_return (s, vs, crash_error)
     end
   end.
 
@@ -548,23 +565,25 @@ Definition run_step_fuel (tt : config_tuple) :=
 Definition run_step d j tt :=
   run_step_with_fuel (run_step_fuel tt) d j tt.
 
-Fixpoint run_v (fuel : fuel) (d : depth) (i : instance) (tt : config_tuple) : ((store_record * res)%type) :=
+Fixpoint run_v (fuel : fuel) (d : depth) (i : instance) (tt : config_tuple)
+    : host_monad (store_record * res) :=
   let: (s, vs, es) := tt in
   match fuel with
-  | 0 => (s, R_crash C_exhaustion)
+  | 0 => host_return (s, R_crash C_exhaustion)
   | fuel.+1 =>
     if es_is_trap es
-    then (s, R_trap)
+    then host_return (s, R_trap)
     else
       if const_list es
-      then (s, R_value (fst (split_vals_e es)))
+      then host_return (s, R_value (fst (split_vals_e es)))
       else
-        let: (s', vs', res) := run_step d i (s, vs, es) in
-        match res with
-        | RS_normal es' => run_v fuel d i (s', vs', es')
-        | RS_crash error => (s, R_crash error)
-        | _ => (s, R_crash C_error)
-        end
+        host_bind (run_step d i (s, vs, es)) (fun rs =>
+          let: (s', vs', res) := rs in
+          match res with
+          | RS_normal es' => run_v fuel d i (s', vs', es')
+          | RS_crash error => host_return (s, R_crash error)
+          | _ => host_return (s, R_crash C_error)
+          end)
   end.
 
 End Host.
@@ -577,8 +596,6 @@ serialise_i64 : i64 -> bytes
 serialise_i32 : i32 -> bytes
 serialise_f64 : f64 -> bytes
 serialise_f32 : f32 -> bytes
-wasm.host : eqType
-(* Some [Equality.axiom] in the wasm module. *)
 Classical_Prop.classic : forall P : Prop, P \/ ~ P
 (* A whole bunch of axioms.  It seems that they come from Flocq, mainly as an axiomatisation of [R].
   Just that we can see things like classical logic and so on. *)
